

$$\begin{aligned}
& \int \frac{8+t+6t^2-12t^3}{(3t^2+4)(t^2+7)} dt \\
& \frac{8+t+6t^2-12t^3}{(3t^2+4)(t^2+7)} = \frac{At+B}{3t^2+4} + \frac{Ct+D}{t^2+7} \\
\implies 8+t+6t^2-12t^3 &= (At+B)(t^2+7) + (Ct+D)(3t^2+4) \\
&= (A+3C)t^3 + (B+3D)t^2 + (7A+4C)t + (7B+4D) \\
&A+3C = -12 \\
&B+3D = 6 \\
&7A+4C = 1 \\
&7B+4D = 8
\end{aligned}$$

$$\begin{aligned}
& \begin{pmatrix} 1 & 3 \\ 7 & 4 \end{pmatrix}^{-1} = \frac{-1}{17} \begin{pmatrix} 4 & -3 \\ -7 & 1 \end{pmatrix} \\
& \begin{pmatrix} 1 & 3 \\ 7 & 4 \end{pmatrix} \begin{pmatrix} A \\ C \end{pmatrix} = \begin{pmatrix} -12 \\ 1 \end{pmatrix} \implies \begin{pmatrix} A \\ C \end{pmatrix} = \begin{pmatrix} 5 \\ 5 \end{pmatrix} \\
& \begin{pmatrix} 1 & 3 \\ 7 & 4 \end{pmatrix} \begin{pmatrix} B \\ D \end{pmatrix} = \begin{pmatrix} 6 \\ 8 \end{pmatrix} \implies \begin{pmatrix} B \\ D \end{pmatrix} = \begin{pmatrix} 0 \\ 2 \end{pmatrix} \\
& = \frac{3t}{3t^2+4} dt + \int \frac{5t}{t^2+7} dt + \int \frac{2}{t^2+7} dt
\end{aligned}$$

$$\int \frac{8+t+6t^2-12t^3}{(3t^2+4)(t^2+7)} dt$$

$$\frac{8+t+6t^2-12t^3}{(3t^2+4)(t^2+7)} = \frac{At+B}{3t^2+4} + \frac{Ct+D}{t^2+7}$$

$$\implies 8+t+6t^2-12t^3 = (At+B)(t^2+7) + (Ct+D)(3t^2+4)$$

$$\text{Let } t^2 = -7$$

$$8+t+6t^2-12t^3 = (At+B)(t^2+7) + (Ct+D)(3t^2+4)$$

$$\implies 8+t-42+84t = (Ct+D)(-17)$$

$$\implies -17C = 85, \quad -17D = -34$$

$$\implies C = -5, \quad D = 2$$

$$\text{Let } t^2 = -\frac{4}{3}$$

$$8+t-8+16t = (At+B)\left(-\frac{4}{3}+7\right)$$

$$\implies 17t = (At+B)\left(\frac{17}{3}\right)$$

$$\implies \frac{17}{3}A = 17, \quad \frac{17}{3}B = 0$$

$$\implies A = 3, \quad B = 0$$

$$= \frac{3t}{3t^2+4} dt + \int \frac{5t}{t^2+7} dt + \int \frac{2}{t^2+7} dt$$